Actualizado

MathCompCurry2.v
@@ -17,54 +17,54 @@ Fixpoint atm_en (s : Term) (j : nat) : Prop :=
   | s1 ∧ s2 => atm_en s1 j \/ atm_en s2 j
   end.
 
-Fixpoint leq (s t : Term) : Prop :=
+Fixpoint sleq (s t : Term) : Prop :=
   match t with
   | Var j => atm_en s j
-  | t1 ∧ t2 => leq s t1 /\ leq s t2
+  | t1 ∧ t2 => sleq s t1 /\ sleq s t2
   end.
-Notation "x ≤ y" := (leq x y)(at level 50).
+Notation "x ≤ y" := (sleq x y)(at level 50).
 
-Structure lattice := Lattice
+Structure semiLattice := SemiLattice
   {
-    reflexq : reflexive leq;
-    antisymq : antisymetric leq;
-    transq : transitive leq;
-    LambdaK : forall a b : Term, leq (a ∧ b) a;
-    LambdaK' : forall a b : Term, leq (a ∧ b) b;
-    LambdaS : forall a b c : Term, (leq c a /\ leq c b ) -> leq c (a ∧ b);
+    reflexq : reflexive sleq;
+    antisymq : antisymetric sleq;
+    transq : transitive sleq;
+    SLambdaK : forall a b : Term, sleq (a ∧ b) a;
+    SLambdaK' : forall a b : Term, sleq (a ∧ b) b;
+    SLambdaS : forall a b c : Term, (sleq c a /\ sleq c b ) -> sleq c (a ∧ b);
    }.
 
-Variable L : lattice.
-Notation ρ := (reflexq L).
-Notation τ := (transq L).
-Notation σ := (antisymq L).
-Notation ΛK := (@LambdaK L).
-Notation ΛK' := (@LambdaK' L).
-Notation ΛS := (@LambdaS L).
+Variable SL : semiLattice.
+Notation Sρ := (reflexq SL).
+Notation Sτ := (transq SL).
+Notation Sσ := (antisymq SL).
+Notation SΛK := (@SLambdaK SL).
+Notation SΛK' := (@SLambdaK' SL).
+Notation SΛS := (@SLambdaS SL).
 
 Theorem ΛW : forall a : Term, a ≤ (a ∧ a).
 Proof.
 move=> a.
-move: (ρ a)=> H0.
-by move: (conj H0 H0)=> /ΛS.
+move: (Sρ a)=> H0.
+by move: (conj H0 H0)=> /SΛS.
 Qed.
 
 Theorem ΛC : forall a b : Term, a ∧ b ≤ b ∧ a.
 Proof.
 move=> a b.
-move: (ΛK' a b)=> H0.
-move: (ΛK a b)=> H1.
-by move: (conj H0 H1)=> /ΛS.
+move: (SΛK' a b)=> H0.
+move: (SΛK a b)=> H1.
+by move: (conj H0 H1)=> /SΛS.
 Qed.
 
 Theorem ΛB : forall a b c : Term, (a ≤ b) -> c ∧ a ≤ c ∧ b.
 Proof.
 move=> a b c H.
-apply: ΛS.
+apply: SΛS.
 split.
-  by apply: ΛK.
-move: (ΛK' c a)=> H0.
-by move: (τ _ _ _ H0 H).
+  by apply: SΛK.
+move: (SΛK' c a)=> H0.
+by move: (Sτ _ _ _ H0 H).
 Qed.
 
 Theorem ΛB' : forall a b c : Term, (a ≤ b) -> a ∧ c ≤ b ∧ c.
@@ -73,36 +73,36 @@ move=> a b c H.
 move: (ΛB a b c)=> /(_ H)-H0.
 move: (ΛC a c)=> H1.
 move: (ΛC c b)=> H2.
-move: (τ _ _ _ H1 H0)=> H3.
-by move: (τ _ _ _ H3 H2).
+move: (Sτ _ _ _ H1 H0)=> H3.
+by move: (Sτ _ _ _ H3 H2).
 Qed.
 
 
-Lemma leqL_atm : forall (n : nat) (s1 s2 : Term),
+Lemma sleqL_atm : forall (n : nat) (s1 s2 : Term),
                (s1 ∧ s2) ≤ Var n <-> atm_en s1 n \/ atm_en s2 n.
 Proof.
 move=> n s1 s2.
-by rewrite /leq /atm_en.
+by rewrite /sleq /atm_en.
 Qed.
 
-Lemma leqR : forall (a t1 t2 : Term), a ≤ (t1 ∧ t2) <-> (a ≤ t1) /\ (a ≤ t2).
+Lemma sleqR : forall (a t1 t2 : Term), a ≤ (t1 ∧ t2) <-> (a ≤ t1) /\ (a ≤ t2).
 Proof.
 move=> a t1 t2.
-by rewrite /leq.
+by rewrite /sleq.
 Qed.
 
 Lemma AtmTerm: forall (n : nat) (a : Term), a ≤ Var n <-> atm_en a n.
 Proof.
 move=> n a.
-by rewrite /leq.
+by rewrite /sleq.
 Qed.
 
 
-Lemma leqL : forall (a b : Term) (n : nat),
+Lemma sleqL : forall (a b : Term) (n : nat),
            a ∧ b ≤ (Var n) <-> a ≤ (Var n) \/ b ≤ (Var n).
 Proof.
 move=> a b n.
-by rewrite leqL_atm -AtmTerm -AtmTerm.
+by rewrite sleqL_atm -AtmTerm -AtmTerm.
 Qed.
 
 
@@ -117,26 +117,26 @@ split; last first.
     rewrite {1}/atm_en => H0.
     by move: H; rewrite H0.
   move=> u Hu v Hv.
-  rewrite leqR.
+  rewrite sleqR.
   move=> [/Hu-H0 /Hv-H1] n0.
   move: (H0 n0) (H1 n0).
   rewrite -AtmTerm -AtmTerm -AtmTerm => H0u H1v.
-  rewrite -AtmTerm leqL.
+  rewrite -AtmTerm sleqL.
   move=> [U | V].
     by move: U => /H0u.
   by move: V => /H1v.
 elim b.
 move=> n H.
   rewrite AtmTerm.
-  by move: (ρ (Var n)) => /AtmTerm /(H n).
+  by move: (Sρ (Var n)) => /AtmTerm /(H n).
 move=> u Hu v Hv Hind.
-rewrite leqR.
+rewrite sleqR.
 split.
   apply: Hu.
   move=> n0.
   rewrite -AtmTerm -AtmTerm => H.
   move: (Hind n0).
-  rewrite -AtmTerm -AtmTerm leqL => H0.
+  rewrite -AtmTerm -AtmTerm sleqL => H0.
   have aux : u ≤ Var n0 \/ v ≤ Var n0. 
     by left.
   by move: aux => /H0.
@@ -144,7 +144,7 @@ apply: Hv.
 move=> n0.
 rewrite -AtmTerm -AtmTerm => H.
 move: (Hind n0).
-rewrite -AtmTerm -AtmTerm leqL => H0.
+rewrite -AtmTerm -AtmTerm sleqL => H0.
 have aux : u ≤ Var n0 \/ v ≤ Var n0.
 by right.
 by move: aux => /H0.
@@ -155,11 +155,11 @@ Proof.
 move=> a.
 have aux: forall i : nat, atm_en (a ∧ a) i -> atm_en a i.
   move=> n.
-  rewrite -AtmTerm -AtmTerm leqL.
+  rewrite -AtmTerm -AtmTerm sleqL.
   by case => H.
-move: aux (ΛK a a) => /Teorema2-H0 H1.
+move: aux (SΛK a a) => /Teorema2-H0 H1.
 move: (conj H1 H0).
-by rewrite σ.
+by rewrite Sσ.
 Qed.
 
 
@@ -169,13 +169,13 @@ move=> a b.
 move: (ΛC b a)=> H0.
 have aux: forall i : nat, atm_en (b ∧ a) i -> atm_en (a ∧ b) i.
   move=> n.
-  rewrite -AtmTerm -AtmTerm leqL leqL.
+  rewrite -AtmTerm -AtmTerm sleqL sleqL.
   case => H.
     by right.
   by left.
 move: aux => /Teorema2-H1.
 move: (conj H0 H1).
-by rewrite σ.
+by rewrite Sσ.
 Qed.
 
 Theorem C3iii : forall a b c : Term, a ∧ (b ∧ c) = (a ∧ b) ∧ c.
@@ -183,8 +183,8 @@ Proof.
 move=> a b c.
 have aux1: forall i : nat, atm_en (a ∧ (b ∧ c)) i -> atm_en ((a ∧ b) ∧ c) i.
   move=> n.
-  rewrite -AtmTerm -AtmTerm leqL leqL.
-  rewrite leqL leqL.
+  rewrite -AtmTerm -AtmTerm sleqL sleqL.
+  rewrite sleqL sleqL.
   move=> [H0 | [H1 | H2]].
       left.
       by left.
@@ -193,8 +193,8 @@ have aux1: forall i : nat, atm_en (a ∧ (b ∧ c)) i -> atm_en ((a ∧ b) ∧ c
   by right.
 have aux2: forall i : nat, atm_en ((a ∧ b) ∧ c) i -> atm_en (a ∧ (b ∧ c)) i.
   move=> n.
-  rewrite -AtmTerm -AtmTerm leqL leqL.
-  rewrite leqL leqL.
+  rewrite -AtmTerm -AtmTerm sleqL sleqL.
+  rewrite sleqL sleqL.
   move=> [[H0 | H1] | H2].
       by left.
     right.
@@ -203,7 +203,7 @@ have aux2: forall i : nat, atm_en ((a ∧ b) ∧ c) i -> atm_en (a ∧ (b ∧ c)
   by right.
 move: aux1 aux2 => /Teorema2-H0 /Teorema2-H1.
 move: (conj H0 H1).
-by rewrite σ.
+by rewrite Sσ.
 Qed.
 
 
@@ -213,16 +213,74 @@ Proof.
 move=> a b.
 split.
   move=> H0.
-  move: (ρ a)=> H1.
-  move:(conj H1 H0)=> /ΛS-H2.
-  move: (ΛK a b) => H3.
-  by move: (conj H2 H3) => /σ.
-rewrite -σ.
+  move: (Sρ a)=> H1.
+  move:(conj H1 H0)=> /SΛS-H2.
+  move: (SΛK a b) => H3.
+  by move: (conj H2 H3) => /Sσ.
+rewrite -Sσ.
 move=> [H0 _].
-move: (ΛK' a b) => H1.
-by move: (τ _ _ _ H0 H1).
+move: (SΛK' a b) => H1.
+by move: (Sτ _ _ _ H0 H1).
 Qed.
 
+Inductive Terms := var (n : nat) | meet (u : Terms) (v : Terms) | join (u : Terms) (v : Terms).
+
+Notation "x ∧ y" := (meet x y) (at level 49). (* \wedge *)
+Notation "x ∨ y" := (join x y) (at level 49). (* \vee*)
+
+Fixpoint auxvt (i : nat) (t : Terms) : Prop :=
+  match t with
+  | var j => i = j
+  | t1 ∧ t2 => (auxvt i t1) /\ (auxvt i t2)
+  | t1 ∨ t2 => (auxvt i t1) \/ (auxvt i t2)
+  end.
+
+Fixpoint auxs (s t : Terms) : Prop :=
+  match s with
+  | var i => auxvt i t
+  | s1 ∧ s2 => (auxs s1 t) \/ (auxs s2 t)
+  | s1 ∨ s2 => (auxs s1 t) /\ (auxs s2 t)
+  end.
+
+Fixpoint atm_enT (j : nat) (s : Terms) : Prop :=
+  match s with
+  | var i => i = j
+  | s1 ∧ s2 => (atm_enT j s1) \/ (atm_enT j s2)
+  | s1 ∨ s2 => (atm_enT j s1) /\ (atm_enT j s2)
+  end.
+
+Fixpoint leq (s t : Terms) : Prop :=
+  match t with
+  | var j => atm_enT j s
+  | t1 ∧ t2 => (leq s t1) /\ (leq s t2)
+  | t1 ∨ t2 => (leq s t1) \/ (leq s t2)
+  end.
+
+Notation "x ≤ y" := (leq x y)(at level 50).
+
+Structure lattice := Lattice
+  {
+    reflexl : reflexive leq;
+    antisyml : antisymetric leq;
+    transl : transitive leq;
+    LambdaK : forall a b : Terms, leq (a ∧ b) a;
+    LambdaK' : forall a b : Terms, leq (a ∧ b) b;
+    LambdaS : forall a b c : Terms, (leq c a /\ leq c b ) -> leq c (a ∧ b);
+    VeK : forall a b : Terms, leq a (a ∨ b);
+    VeK' : forall a b : Terms, leq b (a ∨ b);
+    VeS : forall a b c : Terms, (leq a c /\ leq b c ) -> leq (a ∨ b) c;
+   }.
+
+Variable L : lattice.
+Notation ρ := (reflexl L).
+Notation τ := (transl L).
+Notation σ := (antisyml L).
+Notation ΛK := (@LambdaK L).
+Notation ΛK' := (@LambdaK' L).
+Notation ΛS := (@LambdaS L).
+Notation VK := (@VeK L).
+Notation VK' := (@VeK' L).
+Notation VS := (@VeS L).
 
 
 
